Moved methods

LAB2/Tokeneer/Tokeneer.dfy
@@ -11,12 +11,18 @@ class Token {
 		this.clearanceLevel := clearanceLevel;
 		valid := true;
 	}
+	
+	function method ValidateFingerPrint(scannedFingerprint : int) : bool
+	reads this;
+	{
+		fingerprint == scannedFingerprint
+	}
 }
 
 class Door {
 	var requiredClearanceLevel : int;
 
-	static function method HIGH(): int {3} // Constant are functions that always return the same value
+	static function method HIGH(): int {3} 
 	static function method MEDIUM(): int {2}
 	static function method LOW(): int {1}
 	
@@ -25,6 +31,38 @@ class Door {
 	ensures this.requiredClearanceLevel == requiredClearanceLevel;
 	{
 		this.requiredClearanceLevel := requiredClearanceLevel;
+	}
+	
+	method EnterDoor(user : User) returns (accessGranted : bool)
+	modifies user.token`valid;
+	requires user != null && user.token != null;
+	ensures user.token.valid && user.token.ValidateFingerPrint(user.ScanFinger()) && ValidateClearanceLevel(user.token) ==> accessGranted && user.token.valid;
+	ensures !user.token.valid ==> !accessGranted && !user.token.valid;
+	ensures !user.token.ValidateFingerPrint(user.ScanFinger()) ==> !accessGranted && !user.token.valid;
+	ensures !ValidateClearanceLevel(user.token) ==> !accessGranted;
+	{
+		if (user.token.valid)
+		{
+			var validFingerPrint := user.token.ValidateFingerPrint(user.ScanFinger());
+			if (!validFingerPrint)
+			{
+				user.token.valid := false;
+				accessGranted := false;
+				return;
+			}
+			accessGranted := ValidateClearanceLevel(user.token);
+		}
+		else
+		{
+			accessGranted := false;
+		}
+	}
+	
+	function method ValidateClearanceLevel(token : Token) : bool
+	reads token, this;
+	requires token != null;
+	{
+		token.clearanceLevel >= requiredClearanceLevel
 	}
 }
 
@@ -40,57 +78,16 @@ class User {
 		this.fingerprint := fingerprint;
 		this.token := token;
 	}
+	
+	function method ScanFinger() : int
+	reads this;
+	{
+		fingerprint
+	}
 }
 
 class EnrolmentStation {
 	var users : set<User>; //behövs denna??
-	
-	function method ScanFinger(user : User) : int
-	reads user;
-	requires user != null;
-	{
-		user.fingerprint
-	}
-	
-	function method ValidateFingerPrint(token : Token, scannedFingerprint : int) : bool
-	reads token;
-	requires token != null;
-	{
-		token.fingerprint == scannedFingerprint
-	}
-	
-	function method ValidateClearanceLevel(token : Token, door : Door) : bool
-	reads token, door;
-	requires token != null;
-	requires door != null;
-	{
-		token.clearanceLevel >= door.requiredClearanceLevel
-	}
-  
-	method EnterDoor(user : User, door : Door) returns (accessGranted : bool)
-	modifies user.token`valid;
-	requires user != null && user.token != null && door != null;
-	ensures user.token.valid && ValidateFingerPrint(user.token, ScanFinger(user)) && ValidateClearanceLevel(user.token, door) ==> accessGranted && user.token.valid;
-	ensures !user.token.valid ==> !accessGranted && !user.token.valid;
-	ensures !ValidateFingerPrint(user.token, ScanFinger(user)) ==> !accessGranted && !user.token.valid;
-	ensures !ValidateClearanceLevel(user.token, door) ==> !accessGranted;
-	{
-		if (user.token.valid)
-		{
-			var validFingerPrint := ValidateFingerPrint(user.token, ScanFinger(user));
-			if (!validFingerPrint)
-			{
-				user.token.valid := false;
-				accessGranted := false;
-				return;
-			}
-			accessGranted := ValidateClearanceLevel(user.token, door);
-		}
-		else
-		{
-			accessGranted := false;
-		}
-	}
 	
 	method PrintAccess(accessGranted : bool, tokenValid : bool)
 	{
@@ -123,35 +120,35 @@ class EnrolmentStation {
 		var enrolmentStation := new EnrolmentStation;
 		
 		var user1 := new User.Init(1, token1);
-		var accessGranted := enrolmentStation.EnterDoor(user1, door1);
-		print "user1 with right fingerprint tries to access door1 with token1 (Clearance level enough):\n";
+		var accessGranted := door1.EnterDoor(user1);
+		print "user1 with correct fingerprint tries to access door1 with token1 (Clearance level enough):\n";
 		PrintAccess(accessGranted, token1.valid);
 		
 		var user2 := new User.Init(2, token1);
-		accessGranted := enrolmentStation.EnterDoor(user2, door1);
+		accessGranted := door1.EnterDoor(user2);
 		print "user2 with wrong fingerprint tries to access door1 with token1 (Clearance level enough):\n";
 		PrintAccess(accessGranted, token1.valid);
 		
 		var user3 := new User.Init(1, token1);
-		accessGranted := enrolmentStation.EnterDoor(user3, door1);
-		print "user3 with right fingerprint tries to access door1 with token1 again with invalid token (Clearance level enough):\n";
+		accessGranted := door1.EnterDoor(user3);
+		print "user3 with correct fingerprint tries to access door1 with token1 again with invalid token (Clearance level enough):\n";
 		PrintAccess(accessGranted, token1.valid);
 		
 		var token2 := new Token.Init(1, clearanceLevelMedium);
 		
 		var user4 := new User.Init(1, token2);
-		accessGranted := enrolmentStation.EnterDoor(user4, door1);
-		print "user4 with right fingerprint tries to access door1 with token2 (Clearance level to low):\n";
+		accessGranted := door1.EnterDoor(user4);
+		print "user4 with correct fingerprint tries to access door1 with token2 (Clearance level to low):\n";
 		PrintAccess(accessGranted, token2.valid);
 		
 		var door2 := new Door.Init(clearanceLevelMedium);
-		accessGranted := enrolmentStation.EnterDoor(user4, door2);
-		print "user4 with right fingerprint tries to access door2 with token2 (Clearance level enough):\n";
+		accessGranted := door2.EnterDoor(user4);
+		print "user4 with correct fingerprint tries to access door2 with token2 (Clearance level enough):\n";
 		PrintAccess(accessGranted, token2.valid);
 		
 		var door3 := new Door.Init(clearanceLevelLow);
-		accessGranted := enrolmentStation.EnterDoor(user4, door3);
-		print "user4 with right fingerprint tries to access door3 with token2 (Clearance level more than needed):\n";
+		accessGranted := door3.EnterDoor(user4);
+		print "user4 with correct fingerprint tries to access door3 with token2 (Clearance level more than needed):\n";
 		PrintAccess(accessGranted, token2.valid);
 	
 	}
